Experiments/State_Separator_Calculation_Alternative.thy
@@ -1,0 +1,237 @@
+theory State_Separator_Calculation_Alternative
+imports State_Separator
+begin
+
+section \<open>Alternative Method of Calculating r-distinguishable State Pairs with Separators\<close>
+
+subsection \<open>Input Selection Without Early Termination\<close>
+
+function select_inputs_complete :: "(('a \<times> 'b) \<Rightarrow> ('c \<times> 'a) set) \<Rightarrow> 'b list \<Rightarrow> 'a list \<Rightarrow> 'a set \<Rightarrow> ('a \<times> 'b) list \<Rightarrow> ('a \<times> 'b) list" where
+  "select_inputs_complete f inputList [] nodeSet m = m" |
+  "select_inputs_complete f inputList (n#nL) nodeSet m = 
+    (case find_remove_2 (\<lambda> q' x . f (q',x) \<noteq> {} \<and> (\<forall> (y,q'') \<in> f (q',x) . (q'' \<in> nodeSet))) (n#nL) inputList
+          of None            \<Rightarrow> m |
+             Some (q',x,nodeList') \<Rightarrow> select_inputs_complete f inputList nodeList' (insert q' nodeSet) (m@[(q',x)]))"
+  by pat_completeness auto
+termination 
+ apply (relation "measure (\<lambda> (f,iL,nL,nS,m) . length nL)")
+ apply simp
+proof -
+  fix f :: "(('a \<times> 'b) \<Rightarrow> ('c \<times> 'a) set)"
+  fix inputList :: "'b list"
+  fix n :: 'a
+  fix nL :: "'a list" 
+  fix nodeSet :: "'a set"
+  fix m :: "('a \<times> 'b) list" 
+  fix qynL' q ynL' x nL'
+  assume "find_remove_2 (\<lambda>q' x. f (q', x) \<noteq> {} \<and> (\<forall>(y, q'')\<in>f (q', x). q'' \<in> nodeSet)) (n # nL) inputList = Some qynL'"
+     and "(q, ynL') = qynL'"
+     and "(x, nL') = ynL'"
+
+  then have *: "find_remove_2 (\<lambda>q' x. f (q', x) \<noteq> {} \<and> (\<forall>(y, q'')\<in>f (q', x). q'' \<in> nodeSet)) (n # nL) inputList = Some (q,x,nL')"
+    by auto
+
+  have "q \<in> set (n # nL)"
+  and  "nL' = remove1 q (n # nL)"
+    using find_remove_2_set(2,6)[OF *] by simp+
+
+  then have "length nL' < length (n # nL)"
+    using remove1_length by metis
+    
+
+  then show "((f, inputList, nL', insert q nodeSet, m @ [(q, x)]), f, inputList, n # nL, nodeSet, m) \<in> measure (\<lambda>(f, iL, nL, nS, m). length nL)"
+    by auto
+qed
+
+
+
+
+
+
+
+
+subsection \<open>Alternative Calculation\<close>
+
+subsubsection \<open>Canonical Separator Generator\<close>
+
+text \<open>Generalises the concept of a canonical separator for 2 states to an FSM from which a canonical separator for each pair of states can be extracted simply by moving the initial state to that state pair (encased in an Inl constructor)\<close>
+
+lift_definition canonical_separator_generator :: "('a,'b,'c) fsm \<Rightarrow> (('a \<times> 'a) + LR,'b,'c) fsm" is FSM_Impl.canonical_separator_complete'
+proof -
+  fix A :: "('a,'b,'c) fsm_impl"
+  assume "well_formed_fsm A"
+
+  then have p1a: "fsm_impl.initial A \<in> fsm_impl.nodes A"
+        and p2a: "finite (fsm_impl.nodes A)"
+        and p3a: "finite (fsm_impl.inputs A)"
+        and p4a: "finite (fsm_impl.outputs A)"
+        and p5a: "finite (fsm_impl.transitions A)"
+        and p6a: "(\<forall>t\<in>fsm_impl.transitions A.
+            t_source t \<in> fsm_impl.nodes A \<and>
+            t_input t \<in> fsm_impl.inputs A \<and> t_target t \<in> fsm_impl.nodes A \<and>
+                                             t_output t \<in> fsm_impl.outputs A)"        
+    by simp+
+
+  let ?P = "FSM_Impl.canonical_separator_complete' A"
+
+  show "well_formed_fsm ?P" 
+  proof -
+    
+    let ?f = "(\<lambda>qx . (case (set_as_map (image (\<lambda>(q,x,y,q') . ((q,x),y)) (fsm_impl.transitions A))) qx of Some yqs \<Rightarrow> yqs | None \<Rightarrow> {}))"
+  
+    have "\<And> qx . (\<lambda>qx . (case (set_as_map (image (\<lambda>(q,x,y,q') . ((q,x),y)) (fsm_impl.transitions A))) qx of Some yqs \<Rightarrow> yqs | None \<Rightarrow> {})) qx = (\<lambda> qx . {z. (qx, z) \<in> (\<lambda>(q, x, y, q'). ((q, x), y)) ` fsm_impl.transitions A}) qx"
+    proof -
+      fix qx
+      show "\<And> qx . (\<lambda>qx . (case (set_as_map (image (\<lambda>(q,x,y,q') . ((q,x),y)) (fsm_impl.transitions A))) qx of Some yqs \<Rightarrow> yqs | None \<Rightarrow> {})) qx = (\<lambda> qx . {z. (qx, z) \<in> (\<lambda>(q, x, y, q'). ((q, x), y)) ` fsm_impl.transitions A}) qx"
+        unfolding set_as_map_def by (cases "\<exists>z. (qx, z) \<in> (\<lambda>(q, x, y, q'). ((q, x), y)) ` fsm_impl.transitions A"; auto)
+    qed
+    moreover have "\<And> qx . (\<lambda> qx . {z. (qx, z) \<in> (\<lambda>(q, x, y, q'). ((q, x), y)) ` fsm_impl.transitions A}) qx = (\<lambda> qx . {y | y . \<exists> q' . (fst qx, snd qx, y, q') \<in> fsm_impl.transitions A}) qx"
+    proof -
+      fix qx 
+      show "(\<lambda> qx . {z. (qx, z) \<in> (\<lambda>(q, x, y, q'). ((q, x), y)) ` fsm_impl.transitions A}) qx = (\<lambda> qx . {y | y . \<exists> q' . (fst qx, snd qx, y, q') \<in> fsm_impl.transitions A}) qx"
+        by force
+    qed
+    ultimately have *:" ?f = (\<lambda> qx . {y | y . \<exists> q' . (fst qx, snd qx, y, q') \<in> fsm_impl.transitions A})" 
+      by blast
+      
+  
+    let ?AA = "FSM_Impl.product A A"
+    let ?shifted_transitions' = "shifted_transitions (fsm_impl.transitions ?AA)"
+    let ?distinguishing_transitions_lr = "distinguishing_transitions_LR ?f (fsm_impl.nodes ?AA) (fsm_impl.inputs ?AA)"
+    let ?ts = "?shifted_transitions' \<union> ?distinguishing_transitions_lr"
+
+
+  
+    have pAA: "well_formed_fsm ?AA"
+      using p1a p2a p3a p4a p5a p6a unfolding product_code_naive by fastforce
+
+
+    have "FSM_Impl.nodes ?P = (image Inl (FSM_Impl.nodes ?AA)) \<union> {Inr Left, Inr Right}"
+    and  "FSM_Impl.transitions ?P = ?ts"
+      by simp+
+  
+    
+  
+    
+    have p2: "finite (fsm_impl.nodes ?P)"
+      using pAA unfolding \<open>FSM_Impl.nodes ?P = (image Inl (FSM_Impl.nodes ?AA)) \<union> {Inr Left, Inr Right}\<close> by auto
+
+    have "fsm_impl.initial ?P = Inl (fsm_impl.initial ?AA)" 
+      by auto
+    then have p1: "fsm_impl.initial ?P \<in> fsm_impl.nodes ?P" 
+      using p1a unfolding canonical_separator'.simps by auto
+    have p3: "finite (fsm_impl.inputs ?P)"
+      using p3a by auto
+    have p4: "finite (fsm_impl.outputs ?P)"
+      using p4a by auto
+
+
+    have "finite (fsm_impl.nodes ?AA \<times> fsm_impl.inputs ?AA)"
+      using pAA by auto
+    moreover have **: "\<And> x q1 . finite ({y |y. \<exists>q'. (fst (q1, x), snd (q1, x), y, q') \<in> fsm_impl.transitions A})"
+    proof - 
+      fix x q1
+      have "{y |y. \<exists>q'. (fst (q1, x), snd (q1, x), y, q') \<in> fsm_impl.transitions A} = {t_output t | t . t \<in> fsm_impl.transitions A \<and> t_source t = q1 \<and> t_input t = x}"
+        by auto
+      then have "{y |y. \<exists>q'. (fst (q1, x), snd (q1, x), y, q') \<in> fsm_impl.transitions A} \<subseteq> image t_output (fsm_impl.transitions A)"
+        unfolding fst_conv snd_conv by blast
+      moreover have "finite (image t_output (fsm_impl.transitions A))"
+        using p5a by auto
+      ultimately show "finite ({y |y. \<exists>q'. (fst (q1, x), snd (q1, x), y, q') \<in> fsm_impl.transitions A})"
+        by (simp add: finite_subset)
+    qed
+    ultimately have "finite ?distinguishing_transitions_lr"
+      unfolding * distinguishing_transitions_LR_def by force
+    moreover have "finite ?shifted_transitions'"
+      using pAA unfolding shifted_transitions_def by auto
+    ultimately have "finite ?ts" 
+      by blast
+    then have p5: "finite (fsm_impl.transitions ?P)"
+      by simp
+  
+    
+    have "fsm_impl.inputs ?P = fsm_impl.inputs A"
+      by auto
+    have "fsm_impl.outputs ?P = fsm_impl.outputs A"
+      by auto
+  
+
+    have "\<And> t . t \<in> ?shifted_transitions' \<Longrightarrow> t_source t \<in> fsm_impl.nodes ?P \<and> t_target t \<in> fsm_impl.nodes ?P"
+      using pAA unfolding \<open>FSM_Impl.nodes ?P = (image Inl (FSM_Impl.nodes ?AA)) \<union> {Inr Left, Inr Right}\<close> shifted_transitions_def by auto
+    moreover have "\<And> t . t \<in> ?distinguishing_transitions_lr \<Longrightarrow> t_source t \<in> fsm_impl.nodes ?P \<and> t_target t \<in> fsm_impl.nodes ?P"
+      using pAA unfolding \<open>FSM_Impl.nodes ?P = (image Inl (FSM_Impl.nodes ?AA)) \<union> {Inr Left, Inr Right}\<close> distinguishing_transitions_LR_def * by force
+    ultimately have "\<And> t . t \<in> ?ts \<Longrightarrow> t_source t \<in> fsm_impl.nodes ?P \<and> t_target t \<in> fsm_impl.nodes ?P"
+      by blast
+    moreover have "\<And> t . t \<in> ?shifted_transitions' \<Longrightarrow> t_input t \<in> fsm_impl.inputs ?P \<and> t_output t \<in> fsm_impl.outputs ?P"
+    proof -
+      have "\<And> t . t \<in> ?shifted_transitions' \<Longrightarrow> t_input t \<in> fsm_impl.inputs ?AA \<and> t_output t \<in> fsm_impl.outputs ?AA"
+        using pAA unfolding shifted_transitions_def by auto
+      then show "\<And> t . t \<in> ?shifted_transitions' \<Longrightarrow> t_input t \<in> fsm_impl.inputs ?P \<and> t_output t \<in> fsm_impl.outputs ?P"
+        using pAA unfolding \<open>fsm_impl.inputs ?P = fsm_impl.inputs A\<close> \<open>fsm_impl.outputs ?P = fsm_impl.outputs A\<close> by auto
+    qed
+    moreover have "\<And> t . t \<in> ?distinguishing_transitions_lr \<Longrightarrow> t_input t \<in> fsm_impl.inputs ?P \<and> t_output t \<in> fsm_impl.outputs ?P"
+      unfolding * distinguishing_transitions_LR_def using p6a pAA by auto
+    ultimately have p6: "(\<forall>t\<in>fsm_impl.transitions ?P.
+              t_source t \<in> fsm_impl.nodes ?P \<and>
+              t_input t \<in> fsm_impl.inputs ?P \<and> t_target t \<in> fsm_impl.nodes ?P \<and>
+                                               t_output t \<in> fsm_impl.outputs ?P)"
+      unfolding \<open>FSM_Impl.transitions ?P = ?ts\<close> by blast
+  
+    show "well_formed_fsm ?P"
+      using p1 p2 p3 p4 p5 p6 by linarith
+  qed
+qed 
+
+
+value "canonical_separator m_ex_H 1 2"
+value "canonical_separator_generator m_ex_H"
+
+
+
+
+definition s_states_generator :: "('a::linorder,'b::linorder,'c) fsm \<Rightarrow> ((('a \<times> 'a) + LR) \<times> 'b) list" where
+  "s_states_generator M = (let CG = canonical_separator_generator M
+   in select_inputs_complete (h CG) (inputs_as_list CG) (remove1 (Inr Left) (remove1 (Inr Right) (nodes_as_list CG))) {Inr Left, Inr Right} [])"
+
+value "s_states_generator m_ex_H"
+
+
+
+definition state_separator_generator_from_input_choices :: "('a,'b,'c) fsm \<Rightarrow> (('a \<times> 'a) + LR,'b,'c) fsm \<Rightarrow> ((('a \<times> 'a) + LR) \<times> 'b) list \<Rightarrow> (('a \<times> 'a) + LR, 'b, 'c) fsm" where
+  "state_separator_generator_from_input_choices M CG cs = 
+    (let css  = set cs;
+         cssQ = (set (map fst cs)) \<union> {Inr Left, Inr Right};
+         S0   = filter_nodes CG (\<lambda> q . q \<in> cssQ);
+         S1   = filter_transitions S0 (\<lambda> t . (t_source t, t_input t) \<in> css)          
+    in S1)"
+
+definition state_separators_from_s_states_generator :: "('a::linorder,'b::linorder,'c) fsm \<Rightarrow> (('a \<times> 'a) \<times> ((('a \<times> 'a) + LR, 'b, 'c) fsm)) list" where
+  "state_separators_from_s_states_generator M = 
+    (let 
+          CG = canonical_separator_generator M;
+          cs = filter (\<lambda> (qq,x) . case qq of (Inl (q1,q2)) \<Rightarrow> q1 < q2 | _ \<Rightarrow> False) (s_states_generator M);
+          SG = state_separator_generator_from_input_choices M CG cs         
+    in 
+      concat (map (\<lambda> (qq,x) . case qq of (Inl (q1,q2)) \<Rightarrow> [((q1,q2), from_FSM SG (Inl (q1,q2))),((q2,q1), from_FSM SG (Inl (q1,q2)))] | _ \<Rightarrow> [] ) cs))"
+
+
+
+
+
+definition state_separator_from_s_states :: "('a::linorder,'b::linorder,'c::linorder) fsm \<Rightarrow> 'a \<Rightarrow> 'a \<Rightarrow> (('a \<times> 'a) + 'a, 'b, 'c) fsm option" where
+  "state_separator_from_s_states M q1 q2 = 
+    (let cs = s_states M q1 q2 
+      in (case length cs of
+            0 \<Rightarrow> None |
+            _ \<Rightarrow> if fst (last cs) = Inl (q1,q2)
+                  then Some (state_separator_from_input_choices M (canonical_separator M q1 q2) q1 q2 cs)
+                  else None))"
+
+definition r_distinguishable_state_pairs_with_separators :: "('a::linorder,'b::linorder,'c::linorder) fsm \<Rightarrow> (('a \<times> 'a) \<times> (('a \<times> 'a) + 'a,'b,'c) fsm) set" where
+  "r_distinguishable_state_pairs_with_separators M = {((q1,q2),Sep) | q1 q2 Sep . q1 \<in> nodes M 
+                                                                                \<and> q2 \<in> nodes M 
+                                                                                \<and> ((q1 < q2 \<and> state_separator_from_s_states M q1 q2 = Some Sep)
+                                                                                  \<or> (q2 < q1 \<and> state_separator_from_s_states M q2 q1 = Some Sep)) }"
+
+
+end 
